Cook_Levin_IMP/Views/Examples/Elemof.thy
@@ -2,24 +2,20 @@
 theory Elemof
   imports
     Cook_Levin_IMP.Primitives_IMP_Minus
-    While_To_IMP_Minus_Tactics
+    Cook_Levin_IMP.Compile_Nat
+    IMP_Minus_Views.While_To_IMP_Minus_Locale
+    IMP_Minus_Views.While_To_IMP_Minus_Tactics
 begin
 
-lemma elemof_IMP_loop_body_correct:
-  assumes "(invoke_subprogram p elemof_IMP_loop_body, s) \<Rightarrow>\<^bsup>t\<^esup> s'"
-  shows "elemof_imp_to_HOL_state p s' =
-    elemof_state_upd (elemof_imp_to_HOL_state p s)"
-  apply (insert assms)
-  apply (tactic \<open>HEADGOAL (IMP_start_tac @{cterm "add_prefix p ` elemof_IMP_vars"}
-    @{thm elemof_state_upd_def} @{thm elemof_IMP_loop_body_def}
+lemma elemof_IMP_Minus_loop_body_correct_time:
+  "(invoke_subprogram p elemof_IMP_loop_body, s) \<Rightarrow>\<^bsup>t\<^esup> s' \<Longrightarrow>
+     t = elemof_state_upd_time 0 (elemof_imp_to_HOL_state p s)"
+  by (tactic \<open>HEADGOAL (While_To_IMP_Minus_Tactics.IMP_Minus_run_finish_tac'
+    @{thm elemof_state_upd_time_def} @{thm elemof_IMP_loop_body_def}
+    @{thm elemof_imp_to_HOL_state_def}
+    [(@{thm tl_IMP_Minus_correct}, @{thm tl_imp_to_HOL_state_def})]
+    @{cterm "elemof_IMP_vars"} @{cterm p}
     @{context})\<close>)
-  apply (tactic \<open>HEADGOAL (IMP_step_update_view_tac @{cterm elemof_IMP_vars}
-    @{thm tl_IMP_Minus_correct} @{thm tl_imp_to_HOL_state_def}
-    @{context})\<close>)+
-  apply (tactic \<open>HEADGOAL (IMP_finish_state_eq_tac @{thms elemof_state_translators}
-    "Primitives_IMP_Minus.elemof_state"
-    @{context})\<close>)
-  done
 
 interpretation A : While_To_IMP_Minus where
   cond_var = elemof_while_cond and
@@ -27,46 +23,35 @@ interpretation A : While_To_IMP_Minus where
   body_let = elemof_state_upd and
   base_let = elemof_imp_after_loop and
   loop_let = elemof_imp and
-
   cond_imp = elemof_IMP_init_while_cond and
   body_imp = elemof_IMP_loop_body and
   base_imp = elemof_IMP_after_loop and
-
   imp_to_let_state = elemof_imp_to_HOL_state and
   vars = elemof_IMP_vars
   apply unfold_locales
-  subgoal
-    apply (simp add: elemof_imp_to_HOL_state_def)
-    done
-  subgoal
-    apply auto
-    done
-  subgoal
-    apply (auto simp: elemof_complete_simps)
-    done
-  subgoal
-    apply (fact elemof_IMP_loop_body_correct)
+  subgoal by (simp add: elemof_imp_to_HOL_state_def)
+  subgoal by auto
+  subgoal by (auto simp: elemof_complete_simps)
+  subgoal for s t s' p
+    apply (tactic \<open>HEADGOAL (While_To_IMP_Minus_Tactics.IMP_Minus_run_finish_tac'
+      @{thm elemof_state_upd_def} @{thm elemof_IMP_loop_body_def}
+      @{thm elemof_imp_to_HOL_state_def}
+      [(@{thm tl_IMP_Minus_correct}, @{thm tl_imp_to_HOL_state_def})]
+      @{cterm "elemof_IMP_vars"} @{cterm p}
+      @{context})\<close>)
     done
   subgoal for s t s' p
-    apply (tactic \<open>HEADGOAL (IMP_start_tac @{cterm "add_prefix p ` elemof_IMP_vars"}
+    apply (tactic \<open>HEADGOAL (While_To_IMP_Minus_Tactics.IMP_Minus_run_finish_tac (resolve0_tac @{thms conjI})
       @{thm elemof_imp_compute_loop_condition_def} @{thm elemof_IMP_init_while_cond_def}
+      @{thm elemof_imp_to_HOL_state_def}
+      [
+        (@{thm hd_IMP_Minus_correct}, @{thm hd_imp_to_HOL_state_def}),
+        (@{thm NOTEQUAL_neq_zero_IMP_Minus_correct}, @{thm NOTEQUAL_neq_zero_imp_to_HOL_state_def}),
+        (@{thm AND_neq_zero_IMP_Minus_correct}, @{thm AND_neq_zero_imp_to_HOL_state_def})
+      ]
+      @{cterm "elemof_IMP_vars"} @{cterm p}
       @{context})\<close>)
-    apply (tactic \<open>HEADGOAL (IMP_step_update_view_tac @{cterm elemof_IMP_vars}
-      @{thm hd_IMP_Minus_correct} @{thm hd_imp_to_HOL_state_def}
-      @{context})\<close>)+
-    apply (tactic \<open>HEADGOAL (IMP_step_update_view_tac @{cterm elemof_IMP_vars}
-      @{thm NOTEQUAL_neq_zero_IMP_Minus_correct} @{thm NOTEQUAL_neq_zero_imp_to_HOL_state_def}
-      @{context})\<close>)+
-    apply (tactic \<open>HEADGOAL (IMP_step_update_view_tac @{cterm elemof_IMP_vars}
-      @{thm AND_neq_zero_IMP_Minus_correct} @{thm AND_neq_zero_imp_to_HOL_state_def}
-      @{context})\<close>)+
-    apply (rule conjI;
-      tactic \<open>HEADGOAL (IMP_finish_state_tac @{thms elemof_state_translators}
-        "Primitives_IMP_Minus.elemof_state"
-        @{context})\<close>)
     done
-  using elemof_imp.induct elemof_imp.simps
-    apply auto
-  done
+  using elemof_imp.induct elemof_imp.simps by auto
 
 end
