Cook_Levin_IMP/Views/Examples/Filter_Defined_Acc.thy
@@ -2,42 +2,26 @@
 theory Filter_Defined_Acc
   imports
     Filter_Defined_Acc_Base
-    While_To_IMP_Minus_Tactics
+    IMP_Minus_Views.While_To_IMP_Minus_Locale
+    IMP_Minus_Views.While_To_IMP_Minus_Tactics
 begin
 
-lemma filter_defined_acc_IMP_loop_body_correct:
+lemma filter_defined_acc_IMP_Minus_loop_body_correct:
   assumes "(invoke_subprogram p filter_defined_acc_IMP_loop_body, s) \<Rightarrow>\<^bsup>t\<^esup> s'"
   shows "filter_defined_acc_imp_to_HOL_state p s' =
     filter_defined_acc_state_upd (filter_defined_acc_imp_to_HOL_state p s)"
   apply (insert assms)
-  apply (tactic \<open>HEADGOAL (IMP_start_tac @{cterm "add_prefix p ` filter_defined_acc_IMP_vars"}
+  apply (tactic \<open>HEADGOAL (While_To_IMP_Minus_Tactics.IMP_Minus_run_finish_tac'
     @{thm filter_defined_acc_state_upd_def} @{thm filter_defined_acc_IMP_loop_body_def}
+    @{thm filter_defined_acc_imp_to_HOL_state_def}
+    [
+      (@{thm hd_IMP_Minus_correct}, @{thm hd_imp_to_HOL_state_def}),
+      (@{thm tl_IMP_Minus_correct}, @{thm tl_imp_to_HOL_state_def}),
+      (@{thm cons_IMP_Minus_correct}, @{thm cons_imp_to_HOL_state_def}),
+      (@{thm map_list_find_aux_IMP_Minus_correct}, @{thm map_list_find_aux_imp_to_HOL_state_def})
+    ]
+    @{cterm "filter_defined_acc_IMP_vars"} @{cterm p}
     @{context})\<close>)
-  apply (tactic \<open>HEADGOAL (IMP_step_update_view_tac @{cterm filter_defined_acc_IMP_vars}
-    @{thm hd_IMP_Minus_correct} @{thm hd_imp_to_HOL_state_def}
-    @{context})\<close>)+
-  apply (tactic \<open>HEADGOAL (IMP_step_update_view_tac @{cterm filter_defined_acc_IMP_vars}
-    @{thm map_list_find_aux_IMP_Minus_correct} @{thm map_list_find_aux_imp_to_HOL_state_def}
-    @{context})\<close>)+
-    apply (tactic \<open>HEADGOAL (IMP_if_tac @{thms filter_defined_acc_state_translators} @{context})\<close>)
-    apply (tactic \<open>HEADGOAL (IMP_step_update_view_tac @{cterm filter_defined_acc_IMP_vars}
-      @{thm hd_IMP_Minus_correct} @{thm hd_imp_to_HOL_state_def}
-      @{context})\<close>)+
-    apply (tactic \<open>HEADGOAL (IMP_step_update_view_tac @{cterm filter_defined_acc_IMP_vars}
-      @{thm cons_IMP_Minus_correct} @{thm cons_imp_to_HOL_state_def}
-      @{context})\<close>)+
-    apply (tactic \<open>HEADGOAL (IMP_step_update_view_tac @{cterm filter_defined_acc_IMP_vars}
-      @{thm tl_IMP_Minus_correct} @{thm tl_imp_to_HOL_state_def}
-      @{context})\<close>)+
-    apply (tactic \<open>HEADGOAL (IMP_finish_state_eq_tac @{thms filter_defined_acc_state_translators}
-      "Filter_Defined_Acc_Base.filter_defined_acc_state"
-      @{context})\<close>)
-    apply (tactic \<open>HEADGOAL (IMP_step_update_view_tac @{cterm filter_defined_acc_IMP_vars}
-      @{thm tl_IMP_Minus_correct} @{thm tl_imp_to_HOL_state_def}
-      @{context})\<close>)+
-    apply (tactic \<open>HEADGOAL (IMP_finish_state_eq_tac @{thms filter_defined_acc_state_translators}
-      "Filter_Defined_Acc_Base.filter_defined_acc_state"
-      @{context})\<close>)
   done
 
 interpretation I: While_To_IMP_Minus where
@@ -46,41 +30,42 @@ interpretation I: While_To_IMP_Minus where
   body_let = filter_defined_acc_state_upd and
   base_let = filter_defined_acc_imp_after_loop and
   loop_let = filter_defined_acc_imp and
-
   cond_imp = filter_defined_acc_IMP_init_while_cond and
   body_imp = filter_defined_acc_IMP_loop_body and
   base_imp = filter_defined_acc_IMP_after_loop and
-
   imp_to_let_state = filter_defined_acc_imp_to_HOL_state and
   vars = filter_defined_acc_IMP_vars
   apply unfold_locales
-  subgoal
-    apply (simp add: filter_defined_acc_imp_to_HOL_state_def)
-    done
-  subgoal
-    apply auto
-    done
-  subgoal
-    apply (auto simp: filter_defined_acc_complete_simps filter_defined_acc_IMP_after_loop_def)
-    done
-  subgoal
-    apply (fact filter_defined_acc_IMP_loop_body_correct)
-    done
+  subgoal by (simp add: filter_defined_acc_imp_to_HOL_state_def)
+  subgoal by auto
+  subgoal by (auto simp: filter_defined_acc_complete_simps filter_defined_acc_IMP_after_loop_def)
+  subgoal by (fact filter_defined_acc_IMP_Minus_loop_body_correct)
   subgoal for s t s' p
-    apply (tactic \<open>HEADGOAL (IMP_start_tac @{cterm "add_prefix p ` filter_defined_acc_IMP_vars"}
+    apply (tactic \<open>HEADGOAL (While_To_IMP_Minus_Tactics.IMP_Minus_run_finish_tac (resolve0_tac @{thms conjI})
       @{thm filter_defined_acc_imp_compute_loop_condition_def} @{thm filter_defined_acc_IMP_init_while_cond_def}
+      @{thm filter_defined_acc_imp_to_HOL_state_def}
+      []
+      @{cterm "filter_defined_acc_IMP_vars"} @{cterm p}
       @{context})\<close>)
-    apply (tactic \<open>HEADGOAL (IMP_step_update_view_tac @{cterm filter_defined_acc_IMP_vars}
-      @{thm hd_IMP_Minus_correct} @{thm hd_imp_to_HOL_state_def}
-      @{context})\<close>)+
-    apply (rule conjI;
-      tactic \<open>HEADGOAL (IMP_finish_state_tac @{thms filter_defined_acc_state_translators}
-        "Filter_Defined_Acc_Base.filter_defined_acc_state"
-        @{context})\<close>)
     done
-  using filter_defined_acc_imp.induct filter_defined_acc_imp.simps
-    apply auto
-  done
+  using filter_defined_acc_imp.induct filter_defined_acc_imp.simps by auto
+
+lemma filter_defined_acc_IMP_Minus_loop_body_correct_time:
+  assumes "(invoke_subprogram p filter_defined_acc_IMP_loop_body, s) \<Rightarrow>\<^bsup>t\<^esup> s'"
+  shows "t = filter_defined_acc_state_upd_time 0 (filter_defined_acc_imp_to_HOL_state p s)"
+  apply (insert assms)
+  apply (tactic \<open>HEADGOAL (While_To_IMP_Minus_Tactics.IMP_Minus_run_finish_tac'
+    @{thm filter_defined_acc_state_upd_time_def} @{thm filter_defined_acc_IMP_loop_body_def}
+    @{thm filter_defined_acc_imp_to_HOL_state_def}
+    [
+      (@{thm hd_IMP_Minus_correct}, @{thm hd_imp_to_HOL_state_def}),
+      (@{thm tl_IMP_Minus_correct}, @{thm tl_imp_to_HOL_state_def}),
+      (@{thm cons_IMP_Minus_correct}, @{thm cons_imp_to_HOL_state_def}),
+      (@{thm map_list_find_aux_IMP_Minus_correct}, @{thm map_list_find_aux_imp_to_HOL_state_def})
+    ]
+    @{cterm "filter_defined_acc_IMP_vars"} @{cterm p}
+    @{context})\<close>)
+  oops (*probably an error in the definition of the time function*)
 
 
 end
