Cook_Levin_IMP/Views/While_To_IMP_Minus_Tactics.thy
@@ -1,0 +1,13 @@
+\<^marker>\<open>creator "Kevin Kappelmann"\<close>
+theory While_To_IMP_Minus_Tactics
+  imports
+    Views_Cook_Levin_IMP_Minus
+begin
+          
+lemma Seq_assoc:
+  "((Com.Seq p1 (Com.Seq p2 p3), s) \<Rightarrow>\<^bsup>t\<^esup> s') \<longleftrightarrow> ((Com.Seq (Com.Seq p1 p2) p3, s) \<Rightarrow>\<^bsup>t\<^esup> s')"
+  by auto        
+
+ML_file \<open>while_to_imp_minus_tactics.ML\<close>
+  
+end
